some useful lemmas; fixing errors

SPLean/Experiments/List.lean
@@ -30,20 +30,17 @@ def snd : field := 1
 
 namespace Lang
 
-
+@[simp]
 def MList (L: List val) (p:loc) : hProp :=
   match L with
   | List.nil => ⌜p = null⌝
   | List.cons x L' => ∃ʰ (q:loc), (p ~~~> `{ head := x; tail := q}) ∗ (MList L' q)
 
 lemma MList_nil : ∀ p,
-  (MList List.nil p) = ⌜p = null⌝ :=
-by aesop
+  (MList List.nil p) = ⌜p = null⌝ := by aesop
 
 lemma MList_cons : ∀ p x L',
-  MList (x::L') p = ∃ʰ (q:loc), (p ~~~> `{ head := x; tail := q}) ∗ (MList L' q) :=
-by aesop
-
+  MList (x::L') p = ∃ʰ (q:loc), (p ~~~> `{ head := x; tail := q}) ∗ (MList L' q) := by aesop
 
 lemma MList_if : ∀ (p:loc) (L:List val),
       (MList L p)
@@ -58,26 +55,124 @@ lang_def mnil:= fun u => null
 lemma triple_mnil :
   triple [lang| mnil () ]
   (⌜True⌝)
-  (funloc p ↦ (MList (List.nil) p) ) :=
-by
-  xval
-  xsimp
-  { aesop }
-  { intro; dsimp[MList_nil null]; xsimp }
+  (funloc p ↦ (MList (List.nil) p) ) := by
+  xval; xsimp <;> aesop
 
 
 
-axiom well_founded_ind (A : Type) (R : A -> A -> Prop):
-  ∀ P:A -> Prop,
-    (forall x:A, (forall y:A, R y x -> P y) -> P x) -> ∀ a:A, P a
+--axiom well_founded_ind (A : Type) (R : A -> A -> Prop):
+--  ∀ P:A -> Prop,
+--    (forall x:A, (forall y:A, R y x -> P y) -> P x) -> ∀ a:A, P a
 
 inductive list_sub : (List val) -> (List val) -> Prop where
 | exact (x : val) (L' : List val) : list_sub L' (x::L')
 
 
+def list_sub_Wf : WellFoundedRelation (List val) where
+  rel := list_sub
+  wf  := by
+    constructor
+    intro a
+    induction a with
+    | nil =>
+      constructor
+      intro y H
+      cases H
+    | cons x xs ih =>
+      constructor
+      intro y h
+      cases h; apply ih
+
+
+def measure {α : Type} (f:α->ℕ) : α->α->Prop :=
+  fun x1 x2 => (f x1 < f x2)
+
+
+
+
+def measure_Wf (f:α->ℕ) : WellFoundedRelation α where
+  rel := measure f
+  wf  :=
+  by
+    constructor
+    intro a
+    generalize h : f a = n
+    revert a
+    induction n using Nat.strong_induction_on with
+    | h n' ih =>
+      intro a' hh
+      constructor
+      intro b hhh
+      unfold measure at hhh
+      apply (ih (f b)) <;> aesop
+
+
+-- 0 ≤ m < n.
+def downto0 (m:ℤ) (n:ℤ) : Prop := 0 ≤ m /\ m < n
+
+
+def downto_Wf : WellFoundedRelation ℤ where
+  rel := (downto0)
+  wf  := by
+    constructor
+    intro a
+    induction a using WellFounded.induction (r:= measure (fun n =>  Int.natAbs (n))) with
+    | hwf => apply (measure_Wf (fun n =>  Int.natAbs n)).wf
+    | h x' h =>
+      constructor
+      intro y' H
+      apply h
+      simp[measure]
+      unfold downto0 at H
+      omega
+
+
+def downto0 (m:ℤ) (n:ℤ) : Prop := 0 ≤ m /\ m < n
+
+
+def downto_Wf : WellFoundedRelation ℤ where
+  rel := (downto0)
+  wf  := by
+    constructor
+    intro a
+    induction a using WellFounded.induction (r:= measure (fun n =>  Int.natAbs (n))) with
+    | hwf => apply (measure_Wf (fun n =>  Int.natAbs n)).wf
+    | h x' h =>
+      constructor
+      intro y' H
+      apply h
+      simp[measure]
+      unfold downto0 at H
+      omega
+
+
+def upto (b:ℤ ) :=
+  fun (n m:ℤ ) => (n <= b) /\ (m < n)
+
+
+
+def upto_Wf (b : ℤ): WellFoundedRelation ℤ where
+  rel := upto b
+  wf  := by
+    constructor
+    intro a
+    induction a using WellFounded.induction (r:= measure (fun n =>  Int.natAbs (b-n))) with
+    | hwf => apply (measure_Wf (fun n =>  Int.natAbs (b-n))).wf
+    | h x' h =>
+      constructor
+      intro y' H
+      apply h
+      simp[measure]
+      unfold upto at H
+      omega
+
+
+
+
 
 
 #check tail
+
 
 lang_def append := fix f p1 p2 =>
        let q1 := ⟨val_get_field tail⟩ p1 in
@@ -87,67 +182,85 @@ lang_def append := fix f p1 p2 =>
          else f q1 p2
 
 
-
-
-lemma triple_append (p1 p2 : loc) (L1 L2 : List val): ¬(p1 = null) →
-(triple  [lang| append p1 p2 ] ((MList L1 p1) ∗ (MList L2 p2))
-(fun _ =>  (MList (L1++L2) p1))) :=
-by
-  intro N
-  revert p1
-  induction L1 with
-  | nil =>
-    intro p1 contra
-    xwp
-    xchange (MList_if p1)
-    scase_if
-    {intro H; simp[contra] at H }
-    { intro H; xpull; intro _ _ _ contra; simp at contra }
-  | cons x' L' ih =>
-    intro p1 H
-    xwp
-    xchange (MList_if p1)
-    scase_if
-    { intro H1; simp[H] at H1}
-    { intro H1
-      xpull
-      intro x q1 L1' HH
-      simp at HH
-      simp[HH]
-      xapp triple_get_field_hrecord
+lemma triple_append (p₁ p₂ : loc) (l₁ l₂ : List val) :
+  ¬(p₁ = null) →
+  { MList l₁ p₁ ∗ MList l₂ p₂ }
+    [append p₁ p₂]
+  {_, MList (l₁ ++ l₂) p₁ } := by
+  intros
+  induction l₁ using WellFounded.induction (r:= list_sub) generalizing p₁ with
+  | hwf => apply list_sub_Wf.wf
+  | h l' ih =>
       xwp
-      xchange (MList_if q1)
-      xapp triple_eq
-      simp[is_true]
+      xchange (MList_if p₁)
       scase_if
-      {
-        intro Hq1
-        xif
-        {
-          intro is_true
-          xapp triple_set_field_hrecord
-          simp[MList_cons]
-          xsimp
-        }
-        {
-          intro contra
-          simp at contra
-        }
-      }
-      {
-        intro h
-        xif
-        { intro contra; simp at contra }
-        {
-           intro _
-           xpull
-           intro x_1 q L'_1 hs
-           simp[XSimp]
-           xsimp
-           simp[MList]
-           xapp (ih)
-           simp[hs, MList]
-           xsimp
-        }
-      }
+      {intro _; aesop }
+      intro
+      xsimp; intro x''' q l'' H
+      xapp triple_get_field_hrecord
+      xstep triple_eq
+      xif <;> simp [is_true]
+      { intro; simp [*] at *
+        xapp triple_set_field_hrecord
+        xchange MList_if (L := l'')
+        xsimp; xsimp }
+      intros; xapp H; xsimp
+
+lang_def repeat' := fix g f n =>
+       let b := (n > 0) in
+       if b then
+         f ();
+         let n2 := n - 1 in
+         g f n2 end
+
+#hint_xapp triple_get
+#hint_xapp triple_gt
+#hint_xapp triple_lt
+#hint_xapp triple_sub
+#hint_xapp triple_neq
+
+
+set_option maxHeartbeats 300000
+lemma triple_repeat_aux : ∀ (I:Int → hProp) (f:val) (n:Int),
+  n ≥ 0 →
+  (∀ i, 0 ≤ i /\ i < n →
+    { I i }
+    [ f () ]
+    { _, I (i+1) } ) →
+  (∀ m, 0 ≤ m /\ m ≤ n →
+      { I (n-m) }
+      [ (repeat' f m) ]
+      { _ , I n } ) := by
+  intro I f n Hn Hf m
+  induction m using WellFounded.induction (r:= downto0) with
+  | hwf => apply downto_Wf.wf
+  | h m h =>
+    intro Hm
+    xwp
+    xapp
+    xif <;> intro C
+    { have aux : 0 ≤ (n-m) ∧ (n-m) < n := by aesop
+      xstep Hf (n-m)
+      xwp
+      xapp
+      xapp h
+      have aux1 : n - m + 1 = n - (m-1) := by omega
+      xsimp <;> aesop
+      xsimp <;> aesop
+      simp[downto0]
+      simp at C
+      have aux2 : m >= 1 := by omega
+      simp[aux2]
+      have aux2 : 0 <= m-1 := by omega
+      have aux3 :  m-1 <= n := by omega
+      simp[aux2, aux3]
+    }
+    {
+      simp at C
+      have aux : m = 0 := by omega
+      rw[aux]
+      xsimp
+      aesop
+      xval
+      xsimp
     }
